\documentclass[12pt, letterpaper]{article}
\title {Deriving the derivative of a given expression}
\author{Pavlov Matvey}
\date{\today}
\begin{document}
\maketitle
Function:\[f^{(0)}(x)=\frac{x^2}{x}\]
Taylor decomposition:
\[f(x)=f^{(0)}(x)+ \frac {1}{1!} \cdot f^{(1)}(x)+ \frac {1}{2!} \cdot f^{(2)}(x)+ \frac {1}{3!} \cdot f^{(3)}(x)\]
Substitutions for Taylor:
\[f^{(0)}(x)=\frac{x^2}{x}\]
\[f^{(1)}(x)=A\]
Substitutions:
\[A=\frac{2 \cdot x \cdot x-x^2}{x \cdot x}\]
\[f^{(2)}(x)=\frac{(A) \cdot x \cdot x-B}{x \cdot x \cdot x \cdot x}\]
Substitutions:
\[A=2 \cdot x+2 \cdot x-2 \cdot x\]
\[B=(2 \cdot x \cdot x-x^2) \cdot (x+x)\]
\[f^{(3)}(x)=\frac{(2 \cdot x \cdot x+(A) \cdot (x+x)-(B) \cdot (x+x)+C) \cdot x \cdot x \cdot x \cdot x-((D) \cdot x \cdot x-E) \cdot (F)}{G}\]
Substitutions:
\[A=2 \cdot x+2 \cdot x-2 \cdot x\]
\[B=2 \cdot x+2 \cdot x-2 \cdot x\]
\[C=(2 \cdot x \cdot x-x^2) \cdot 2\]
\[D=2 \cdot x+2 \cdot x-2 \cdot x\]
\[E=(2 \cdot x \cdot x-x^2) \cdot (x+x)\]
\[F=(x+x) \cdot x \cdot x+x \cdot x \cdot (x+x)\]
\[G=x \cdot x \cdot x \cdot x \cdot x \cdot x \cdot x \cdot x\]
\end{document}